theories/Mem.v
@@ -1,0 +1,115 @@
+Require Import Coqlib.
+Require Import ITreelib.
+Require Import Universe.
+Require Import STS.
+Require Import Behavior.
+Require Import ModSem.
+Require Import Skeleton.
+Require Import PCM.
+
+Generalizable Variables E R A B C X Y Z GRA.
+
+Set Implicit Arguments.
+
+
+
+Instance points_to: RA.t := RA.pointwise block (RA.pointwise Z (RA.agree (unit + val))).
+Compute (RA.car).
+
+Definition own {GRA: GRA.t} (whole a: URA.car (t:=GRA)): Prop := URA.extends a whole.
+
+
+(***
+r <- Take;;
+FAdd(r);; <-------------------------- illegal in some sense
+assume((blk |-> R) <= r \/ (blk |-> G) <= r \/ (blk |-> B) <= r);;  (iProp???)
+meta-assume(list mname(for modular reasoning), current stackframe);;
+
+r <- Choose;;
+FSub(r);; := Get;; Choose;; guarantee;; Set;;
+guarantee(blk |-> v <= r);;
+(call f);;
+r <- Take;;
+FAdd(r);; <-------------------------- illegal in some sense
+assume(some_other_resource <= r);;
+meta-assume(list mname(for modular reasoning), current stackframe);;
+
+r <- Choose;;
+FSub(r);;
+guarantee(blk |-> v <= r);;
+***)
+
+(***
+HoareFun := FPush;; [[boilerplate]] real_code [[boilerplate]] FPop;;
+real_code := itree, using HoareCall, not benign call
+             calling meta-assume is allowed. "list mname" is hard-coded in the module.
+HoareCall := [[boilerplate]] call [[boilerplate]]
+
+the illegal update (FAdd(r)) is only allowed in boilerplate code.
+FPush/FPop is only allowed in boilerplate code.
+***)
+
+(***
+FPush
+  r <- Take;
+  assume(P /\ IP r);
+  cur <- FGet; FPut (cur * r);
+
+
+
+    r <- Choose;
+    guarantee(P /\ IP r);
+    cur <- FGet; cur' <- Choose; guarantee(cur' * r = cur); FPut cur';
+      call;
+    ...
+    ...
+    ...
+
+  ...
+  ...
+  ...
+FPop
+
+NB: this "discarded" resource is *actually* discarded; the user can't access it in the real_code
+***)
+
+(***
+Where does the `Function Locality` appear in our scenario?
+1. Write it with assume/guarantee.
+2. Use Rely/Guarantee in simulation technique.
+
+<<<<<<<<<<<<<< Maybe it is better to give function call stack for each mname,
+               for better modularity & less cognitive overhead >>>>>>>>>>>>>>>>>
+
+FPush
+  r <- Take;
+  assume(P /\ IP r);
+  cur <- FGet; FPut (cur * r);
+
+
+
+    r <- Choose;
+    guarantee(P /\ IP r);
+    cur <- FGet; cur' <- Choose; guarantee(cur' * r = cur); FPut cur';
+      call;
+    ...
+    ...
+    ...
+
+  ...
+  ...
+  ...
+FPop
+
+***)
+
+
+
+Local Notation "blk#ofs |-> v" := blk 
+  (at level 20, q at level 50, format "l  ↦{ q }  v") : bi_scope.
+
+Section PROOF.
+  Variable points_to: URA.t.
+  Context `{@GRA.inG points_to GRA}.
+Definition mem: ModSem.t
+End PROOF.
